removing "unlikely to be used" calling conventions

src/ClangPrinter.cpp
@@ -135,25 +135,31 @@ ClangPrinter::printCallingConv(clang::CallingConv cc, CoqPrinter &print) {
     case CallingConv::x:                                                       \
         print.output() << #x;                                                  \
         break;
+#define OVERRIDE(x, y)                                                         \
+    case CallingConv::x:                                                       \
+        print.output() << #y;                                                  \
+        break;
     switch (cc) {
-    PRINT(CC_C);
-    PRINT(CC_X86StdCall);
-    PRINT(CC_X86FastCall);
-    PRINT(CC_X86ThisCall);
-    PRINT(CC_X86VectorCall);
-    PRINT(CC_X86Pascal);
-    PRINT(CC_Win64);
-    PRINT(CC_X86_64SysV);
-    PRINT(CC_X86RegCall);
-    PRINT(CC_AAPCS);
-    PRINT(CC_AAPCS_VFP);
-    PRINT(CC_IntelOclBicc);
-    PRINT(CC_SpirFunction);
-    PRINT(CC_OpenCLKernel);
-    PRINT(CC_Swift);
-    PRINT(CC_PreserveMost);
-    PRINT(CC_PreserveAll);
-    PRINT(CC_AArch64VectorCall);
+        PRINT(CC_C);
+        OVERRIDE(CC_X86RegCall, CC_RegCall);
+        OVERRIDE(CC_Win64, CC_MsAbi);
+#if 0
+        PRINT(CC_X86StdCall);
+        PRINT(CC_X86FastCall);
+        PRINT(CC_X86ThisCall);
+        PRINT(CC_X86VectorCall);
+        PRINT(CC_X86Pascal);
+        PRINT(CC_X86_64SysV);
+        PRINT(CC_AAPCS);
+        PRINT(CC_AAPCS_VFP);
+        PRINT(CC_IntelOclBicc);
+        PRINT(CC_SpirFunction);
+        PRINT(CC_OpenCLKernel);
+        PRINT(CC_Swift);
+        PRINT(CC_PreserveMost);
+        PRINT(CC_PreserveAll);
+        PRINT(CC_AArch64VectorCall);
+#endif
     default:
         using namespace logging;
         logging::fatal() << "unsupported calling convention\n";
